checkpoint converting to module-based nested programs

src/DiskLib.v
@@ -4,7 +4,8 @@ Require Import Closures.
 Require Import Util.
 Require Import Arith.
 Require Import Smallstep.
-Require Import Disk.
+Require Import DiskMod.
+Open Scope fscq.
 
 
 Module Pair <: SmallStepLang.
@@ -82,134 +83,10 @@ Qed.
 End PairToDisk.
 
 
-Module Type DualProgType (Left Right:SmallStepLang) <: SmallStepLang.
-
-(* XXX Module system warts: this weird type seems needed for the RefineDual
- * module below, for two reasons.
- *
- * First, RefineDual needs to refer to (DualProg L1 R1) and (DualProg L2 R2).
- * If RefineDual instantiates these internally, then they appear as different
- * types from instantiations of the same DualProg elsewhere; as a result,
- * programs that are the same appear to have different types.
- *
- * Second, RefineDual satisfies Refine (DualProg L1 R1) (DualProg L2 R2), but
- * specifying that syntax causes Coq to complain that "Application of modules
- * is restricted to paths".
- *
- * Using this type allows passing in "existing" copies of the two DualProg
- * modules, avoiding both problems.
- *
- * Unfortunately, it's a verbatim copy of DualProg..
- *)
-
-Inductive prog {R:Type} : Type :=
-  | DoLeft {T:Type} (p:Left.Prog T) (rx:T->prog)
-  | DoRight {T:Type} (p:Right.Prog T) (rx:T->prog)
-  | Return (r:R).
-Definition Prog := @prog.
-Definition ReturnOp := @Return.
-
-Inductive state :=
-  | DualState (l:Left.State) (r:Right.State).
-Definition State := state.
-
-Inductive step {R:Type} : @progstate R Prog State ->
-                          @progstate R Prog State -> Prop :=
-  | DualStepLeft: forall p rx ls ls' rs r
-    (LS: progreturns (Left.Step R) (Left.ReturnOp R) p ls ls' r),
-    step (PS (DoLeft p rx) (DualState ls rs))
-         (PS (rx r) (DualState ls' rs))
-  | DualStepRight: forall p rx ls rs rs' r
-    (RS: progreturns (Right.Step R) (Right.ReturnOp R) p rs rs' r),
-    step (PS (DoRight p rx) (DualState ls rs))
-         (PS (rx r) (DualState ls rs')).
-Definition Step := @step.
-
-End DualProgType.
 
 
-Module DualProg (Left: SmallStepLang) (Right: SmallStepLang) <: DualProgType Left Right.
-
-Inductive prog {R:Type} : Type :=
-  | DoLeft {T:Type} (p:Left.Prog T) (rx:T->prog)
-  | DoRight {T:Type} (p:Right.Prog T) (rx:T->prog)
-  | Return (r:R).
-Definition Prog := @prog.
-Definition ReturnOp := @Return.
-
-Inductive state :=
-  | DualState (l:Left.State) (r:Right.State).
-Definition State := state.
-
-Inductive step {R:Type} : @progstate R Prog State ->
-                          @progstate R Prog State -> Prop :=
-  | DualStepLeft: forall p rx ls ls' rs r
-    (LS: progreturns (Left.Step R) (Left.ReturnOp R) p ls ls' r),
-    step (PS (DoLeft p rx) (DualState ls rs))
-         (PS (rx r) (DualState ls' rs))
-  | DualStepRight: forall p rx ls rs rs' r
-    (RS: progreturns (Right.Step R) (Right.ReturnOp R) p rs rs' r),
-    step (PS (DoRight p rx) (DualState ls rs))
-         (PS (rx r) (DualState ls rs')).
-Definition Step := @step.
-
-End DualProg.
 
 
-Module RefineDual (L1 R1 L2 R2: SmallStepLang)
-                  (DP1: DualProgType L1 R1)
-                  (DP2: DualProgType L2 R2)
-                  (L12: Refines L1 L2)
-                  (R12: Refines R1 R2) <: Refines DP1 DP2.
-
-Module FSR_L := FSimReturn L1 L2 L12.
-Module FSR_R := FSimReturn R1 R2 R12.
-
-Fixpoint Compile {R:Type} (p:@DP1.Prog R) : @DP2.Prog R :=
-  match p with
-  | DP1.DoLeft T p rx => DP2.DoLeft (L12.Compile T p) (fun x => Compile (rx x))
-  | DP1.DoRight T p rx => DP2.DoRight (R12.Compile T p) (fun x => Compile (rx x))
-  | DP1.Return v => DP2.Return v
-  end.
-
-Inductive statematch : DP1.State -> DP2.State -> Prop :=
-  | Match: forall l1 r1 l2 r2
-    (ML: L12.StateMatch l1 l2)
-    (MR: R12.StateMatch r1 r2),
-    statematch (DP1.DualState l1 r1) (DP2.DualState l2 r2).
-Definition StateMatch := statematch.
-Hint Constructors statematch.
-
-Theorem FSim:
-  forall R,
-  forward_simulation (DP1.Step R) (DP2.Step R).
-Proof.
-  intros; exists (progmatch Compile statematch); intros.
-
-  repeat match goal with
-  | [ x: progmatch _ _ _ _ |- _ ] => inversion x; clear x; subst
-  | [ x: statematch _ _ |- _ ] => inversion x; clear x; subst
-  end.
-
-  match goal with
-  | [ x: DP1.Step _ _ _ |- _ ] => inversion x; clear x; subst
-  end.
-
-  - (* DoLeft *)
-    destruct FSR_L.fsim_implies_returns with
-      (R:=R) (p:=p) (s1:=l1) (s1':=ls') (s2:=l2) (r:=r); auto. Tactics.destruct_pairs.
-    eexists; split.
-    + eapply star_step; [constructor; eauto|apply star_refl].
-    + constructor; [|constructor]; auto.
-  - (* DoRight *)
-    destruct FSR_R.fsim_implies_returns with
-      (R:=R) (p:=p) (s1:=r1) (s1':=rs') (s2:=r2) (r:=r); auto. Tactics.destruct_pairs.
-    eexists; split.
-    + eapply star_step; [constructor; eauto|apply star_refl].
-    + constructor; [|constructor]; auto.
-Qed.
-
-End RefineDual.
 
 
 (* An example of how to write a program in a dual language *)
