src/FsPartsMod.v
@@ -1,0 +1,168 @@
+Require Import CpdtTactics.
+Require Import FsTactics.
+Require Import DiskMod.
+Require Import Util.
+Require Import Smallstep.
+Require Import Closures.
+Require Import Tactics.
+
+
+Module Type FsPartsType
+       (Inode: SmallStepLang)
+       (Bmap: SmallStepLang)
+       (Blocks: SmallStepLang) <: SmallStepLang.
+
+(*
+ * XXX Module system warts: this weird type seems needed for the RefineParts
+ * module below, for two reasons.
+ *
+ * First, RefineParts needs to refer to (FsParts I1 M1 B1) and (FsParts I2 M2 B2).
+ * If RefineParts instantiates these internally, then they appear as different
+ * types from instantiations of the same FsParts elsewhere; as a result,
+ * programs that are the same appear to have different types.  This seems to be
+ * the bigger problem.
+ *
+ * Second, RefineParts satisfies Refine (FsParts I1 M1 B1) (FsParts I2 M2 B2), but
+ * specifying that syntax causes Coq to complain that "Application of modules
+ * is restricted to paths".  This seems less critical; if the first problem above
+ * were solved, we could solve this one by just stating later that it satisfies
+ * the type; modules in Coq do not need to state every type they satisfy upfront.
+ *
+ * This type allows passing in "existing" copies of the two FsParts modules,
+ * avoiding both problems.
+ *
+ * Unfortunately, it's a verbatim copy of FsParts..
+ *)
+
+Inductive prog {R:Type} : Type :=
+  | I {T:Type} (p:Inode.Prog T) (rx:T->prog)
+  | M {T:Type} (p:Bmap.Prog T) (rx:T->prog)
+  | B {T:Type} (p:Blocks.Prog T) (rx:T->prog)
+  | Return (r:R).
+Definition Prog := @prog.
+Definition ReturnOp := @Return.
+
+Inductive state :=
+  | PartState (i:Inode.State) (m:Bmap.State) (b:Blocks.State).
+Definition State := state.
+
+Inductive step {R:Type} : @progstate R Prog State ->
+                          @progstate R Prog State -> Prop :=
+  | StepI: forall p rx s s' m b r
+    (S: progreturns (Inode.Step R) (Inode.ReturnOp R) p s s' r),
+    step (PS (I p rx) (PartState s m b))
+         (PS (rx r) (PartState s' m b))
+  | StepM: forall p rx s s' i b r
+    (S: progreturns (Bmap.Step R) (Bmap.ReturnOp R) p s s' r),
+    step (PS (M p rx) (PartState i s b))
+         (PS (rx r) (PartState i s' b))
+  | StepB: forall p rx s s' i m r
+    (S: progreturns (Blocks.Step R) (Blocks.ReturnOp R) p s s' r),
+    step (PS (B p rx) (PartState i m s))
+         (PS (rx r) (PartState i m s')).
+Definition Step := @step.
+
+End FsPartsType.
+
+
+Module FsParts
+       (Inode: SmallStepLang)
+       (Bmap: SmallStepLang)
+       (Blocks: SmallStepLang) <: FsPartsType Inode Bmap Blocks.
+
+Inductive prog {R:Type} : Type :=
+  | I {T:Type} (p:Inode.Prog T) (rx:T->prog)
+  | M {T:Type} (p:Bmap.Prog T) (rx:T->prog)
+  | B {T:Type} (p:Blocks.Prog T) (rx:T->prog)
+  | Return (r:R).
+Definition Prog := @prog.
+Definition ReturnOp := @Return.
+
+Inductive state :=
+  | PartState (i:Inode.State) (m:Bmap.State) (b:Blocks.State).
+Definition State := state.
+
+Inductive step {R:Type} : @progstate R Prog State ->
+                          @progstate R Prog State -> Prop :=
+  | StepI: forall p rx s s' m b r
+    (S: progreturns (Inode.Step R) (Inode.ReturnOp R) p s s' r),
+    step (PS (I p rx) (PartState s m b))
+         (PS (rx r) (PartState s' m b))
+  | StepM: forall p rx s s' i b r
+    (S: progreturns (Bmap.Step R) (Bmap.ReturnOp R) p s s' r),
+    step (PS (M p rx) (PartState i s b))
+         (PS (rx r) (PartState i s' b))
+  | StepB: forall p rx s s' i m r
+    (S: progreturns (Blocks.Step R) (Blocks.ReturnOp R) p s s' r),
+    step (PS (B p rx) (PartState i m s))
+         (PS (rx r) (PartState i m s')).
+Definition Step := @step.
+
+End FsParts.
+
+
+Module RefineParts (I1 M1 B1: SmallStepLang)
+                   (I2 M2 B2: SmallStepLang)
+                   (P1: FsPartsType I1 M1 B1)
+                   (P2: FsPartsType I2 M2 B2)
+                   (I12: Refines I1 I2)
+                   (M12: Refines M1 M2)
+                   (B12: Refines B1 B2) <: Refines P1 P2.
+
+Module FSR_I := FSimReturn I1 I2 I12.
+Module FSR_M := FSimReturn M1 M2 M12.
+Module FSR_B := FSimReturn B1 B2 B12.
+
+Fixpoint Compile {R:Type} (p:@P1.Prog R) : @P2.Prog R :=
+  match p with
+  | P1.I T p rx => P2.I (I12.Compile T p) (fun x => Compile (rx x))
+  | P1.M T p rx => P2.M (M12.Compile T p) (fun x => Compile (rx x))
+  | P1.B T p rx => P2.B (B12.Compile T p) (fun x => Compile (rx x))
+  | P1.Return v => P2.Return v
+  end.
+
+Inductive statematch : P1.State -> P2.State -> Prop :=
+  | Match: forall i1 i2 m1 m2 b1 b2
+    (MI: I12.StateMatch i1 i2)
+    (MM: M12.StateMatch m1 m2)
+    (MB: B12.StateMatch b1 b2),
+    statematch (P1.PartState i1 m1 b1) (P2.PartState i2 m2 b2).
+Definition StateMatch := statematch.
+Hint Constructors statematch.
+
+Theorem FSim:
+  forall R,
+  forward_simulation (P1.Step R) (P2.Step R).
+Proof.
+  intros; exists (progmatch Compile statematch); intros.
+
+  repeat match goal with
+  | [ x: progmatch _ _ _ _ |- _ ] => inversion x; clear x; subst
+  | [ x: statematch _ _ |- _ ] => inversion x; clear x; subst
+  end.
+
+  match goal with
+  | [ x: P1.Step _ _ _ |- _ ] => inversion x; clear x; subst
+  end.
+
+  - (* I *)
+    destruct FSR_I.fsim_implies_returns with
+      (R:=R) (p:=p) (s1:=i1) (s1':=s') (s2:=i2) (r:=r); auto. Tactics.destruct_pairs.
+    eexists; split.
+    + eapply star_step; [constructor; eauto|apply star_refl].
+    + constructor; [|constructor]; auto.
+  - (* M *)
+    destruct FSR_M.fsim_implies_returns with
+      (R:=R) (p:=p) (s1:=m1) (s1':=s') (s2:=m2) (r:=r); auto. Tactics.destruct_pairs.
+    eexists; split.
+    + eapply star_step; [constructor; eauto|apply star_refl].
+    + constructor; [|constructor]; auto.
+  - (* B *)
+    destruct FSR_B.fsim_implies_returns with
+      (R:=R) (p:=p) (s1:=b1) (s1':=s') (s2:=b2) (r:=r); auto. Tactics.destruct_pairs.
+    eexists; split.
+    + eapply star_step; [constructor; eauto|apply star_refl].
+    + constructor; [|constructor]; auto.
+Qed.
+
+End RefineParts.
